fix matching regs

theories/automation.v
@@ -442,22 +442,42 @@ Section instances.
     Subsume (r # f ↦ᵣ v) (reg_col ((KindField r f, s)::regs)) :=
     λ G, i2p (subsume_struct_reg_regcol regs r f v s G).
 
-  Fixpoint cancel_reg_col (regs1 regs2 : list (reg_kind * valu_shape)) (i2 : nat) : (list (nat * nat)) :=
+  Fixpoint find_matching_regs (regs1 regs2 : list (reg_kind * valu_shape)) (i2 : nat) : (list (nat * nat)) :=
     match regs2 with
     | (r, s)::rs =>
         if list_find_idx (λ x, x.1 = r) regs1 is Some i1 then
-          (i1, i2)::cancel_reg_col (delete i1 regs1) rs (S i2)
+          (i1, i2)::find_matching_regs regs1 rs (S i2)
         else
-          cancel_reg_col regs1 rs (S i2)
+          find_matching_regs regs1 rs (S i2)
     | [] => []
     end.
+  Lemma find_matching_regs_sound regs1 regs2 i2:
+    Forall (λ i, ∃ vr1 vr2, (i2 ≤ i.2)%nat ∧ regs1 !! i.1 = Some vr1 ∧ regs2 !! (i.2 - i2)%nat = Some vr2 ∧ vr1.1 = vr2.1) (find_matching_regs regs1 regs2 i2).
+  Proof.
+    elim: regs2 regs1 i2 => //=.
+    move => [??] regs2 IH regs1 i2. case_match.
+    - apply: Forall_cons.
+      + revert select (list_find_idx _ _ = _) => /list_find_idx_Some[?[?[??]]]; simplify_eq.
+        eexists _, _ => /=. rewrite -minus_n_n /=. done.
+      + apply: Forall_impl; [| by apply: IH].
+        move => [a1 a2] /=[?[?[?[?[??]]]]].
+        eexists _, _. split_and! => //. { lia. }
+        suff -> : (a2 - i2)%nat = S (a2 - S i2)%nat by done. lia.
+    - apply: Forall_impl; [| by apply: IH].
+      move => [a1 a2] /=[?[?[?[?[??]]]]].
+      eexists _, _. split_and! => //. { lia. }
+      suff -> : (a2 - i2)%nat = S (a2 - S i2)%nat by done. lia.
+  Qed.
+
   Lemma subsume_regcol_regcol regs1 regs2 G:
-    (∃ idxs, ⌜(via_vm_compute cancel_reg_col regs1 regs2 0%nat) = idxs⌝ ∗
-       ⌜foldr (λ '(i1,i2), and (valu_shape_implies (regs1 !!! i1).2 (regs2 !!! i2).2)) True idxs⌝ ∗
+    (∃ idxs, ⌜(via_vm_compute find_matching_regs regs1 regs2 0%nat) = idxs⌝ ∗
+       ⌜foldr (λ i, and (valu_shape_implies (regs1 !!! i.1).2 (regs2 !!! i.2).2)) True idxs⌝ ∗
        (reg_col (foldr delete regs1 idxs.*1) -∗ reg_col (foldr delete regs2 idxs.*2) ∗ G)) -∗
     subsume (reg_col regs1) (reg_col regs2) G.
   Proof.
     rewrite via_vm_compute_eq.
+    iIntros "[%idxs [%Hcancel [%Hall HG]]]".
+    move/Forall_fold_right in Hall.
   Admitted.
     (* iDestruct 1 as (i [[??][?[??]]]%list_find_idx_Some) "HG"; simplify_eq/=. iIntros "Hr". *)
     (* rewrite /reg_col. erewrite (delete_Permutation regs); [|done] => /=. *)
